\documentclass[10pt,a4paper]{article}
\usepackage[utf8]{inputenc}
\usepackage[T1]{fontenc}
\usepackage{amsmath}
\usepackage{amsfonts}
\usepackage{amssymb}
\usepackage{graphicx}
\usepackage{xeCJK}
\usepackage{amsmath}

\begin{document}
	

	\begin{equation}
		f(x,n) = \sum_{i=1}^{k}f(x-i,n-1)
	\end{equation}
	\begin{equation}
		f(x-1,n) = \sum_{i=1}^{k}f(x-1-i,n-1)
	\end{equation}
	
	由（1) - (2) 得
		
		\begin{equation}
			f(x,n) = f(x-1,n-1) + f(x-1,n) - f(x-1-k,n-1)
		\end{equation}
	由 （3）  得到
	 \begin{equation}
	 	f(x-1,n) = f(x,n) + f(x-1-k,n-1)  -f(x-1,n)
	 \end{equation}
 
 \begin{equation}
 	f(x,n) = f(x+1,n) + f(x-k,n-1) - f(x,n)
 \end{equation}
	
	
	
	
	
\end{document}